{
 "cells": [
  {
   "cell_type": "markdown",
   "metadata": {},
   "source": [
    "**1. Recall the definition of a rational number, denoted as $\\mathbb{Q}$. Prove that the Euler's number $e = \\Sigma_{k=0}^\\infty \\frac{1}{k!} \\notin \\mathbb{Q}$. A factorial is defined as $k! = (k)(k-1)(k-2)(k-3)..., \\forall k \\in \\mathbb{Z}^+$, note that $0! = 1$. Furthermore, a sum notation $\\Sigma_{k=0}^\\infty k = 0+ 1 + 2 + 3 +....+...$**\n",
    "\n",
    "# Proof by Contradiction:\n",
    "\n",
    "1. Let's start by assuming that Euler's number, $e$, is a rational number. This means we can express $e$ as a fraction $\\frac{p}{q}$, where $p$ and $q$ are integers with no common factors other than 1, and $q \\neq 0$.\n",
    "\n",
    "2. We know that $e$ is defined as the sum of an infinite series: $e = \\Sigma_{k=0}^\\infty \\frac{1}{k!}$.\n",
    "\n",
    "3. Let's consider the partial sums of this series, denoted as $S_n$. As $n$ approaches infinity, these partial sums should converge to a rational limit, since we're assuming $e$ is rational.\n",
    "\n",
    "4. However, each term in the series $\\frac{1}{k!}$ is positive, which means each partial sum $S_n$ is increasing. \n",
    "\n",
    "5. If we look at the factorial terms $k!$, for any $k \\geq 1$, we have $k! > k$, which implies $\\frac{1}{k!} < \\frac{1}{k}$.\n",
    "\n",
    "6. This leads us to the Harmonic series, $\\sum_{k=0}^\\infty \\frac{1}{k}$, which is known to diverge. But since $\\frac{1}{k!} < \\frac{1}{k}$, we can conclude that the series $\\sum_{k=0}^\\infty \\frac{1}{k!}$ converges.\n",
    "\n",
    "7. This is a contradiction, because if $S_n$ converges to a rational number, it must be bounded. But the convergence of $\\sum_{k=0}^\\infty \\frac{1}{k!}$ contradicts the unboundedness of the Harmonic series.\n",
    "\n",
    "# Conclusion:\n",
    "Our assumption that $e$ is rational leads to a contradiction. Therefore, we conclude that $e$ is not rational, i.e., $e \\notin \\mathbb{Q}$.\n",
    "<hr>\n"
   ]
  },
  {
   "cell_type": "markdown",
   "metadata": {},
   "source": [
    "**2. Prove Minkowski's Inequality for sums, $\\forall \\ p>1, (a_k, b_k)>0$ &nbsp;: &nbsp;\n",
    "$\\left( \\sum_{k=1}^n |a_k + b_k|^p \\right)^\\frac{1}{p}$\n",
    "$\\leq$\n",
    "$\\left( \\sum_{k=1}^n |a_k|^p \\right)^\\frac{1}{p}$ +\n",
    "$\\left( \\sum_{k=1}^n |b_k|^p \\right)^\\frac{1}{p}$**\n",
    "\n",
    "# Proof by Contradiction:\n",
    "\n",
    "1. We start by assuming that the inequality $\\left( \\sum_{k=1}^n |a_k + b_k|^p \\right)^{\\frac{1}{p}} > \\left( \\sum_{k=1}^n |a_k|^p\\right)^{\\frac{1}{p}} + \\left( \\sum_{k=1}^n |b_k|^p\\right)^{\\frac{1}{p}}$ holds true.\n",
    "\n",
    "2. This implies that $\\sum_{k=1}^n |a_k + b_k|^p > \\left( \\sum_{k=1}^n |a_k|^p\\right) + \\left( \\sum_{k=1}^n |b_k|^p\\right)$.\n",
    "\n",
    "3. Now, let's consider the function $f(x) = |x|^p$. By applying Hölder’s Inequality, we get $\\sum_{k=1}^n |a_k + b_k|^p \\leq \\left( \\sum_{k=1}^n |a_k|^p\\right)^{\\frac{1}{p}} \\left( \\sum_{k=1}^n |b_k|^p\\right)^{\\frac{1}{p}}$.\n",
    "\n",
    "4. Here, we encounter a contradiction. Our assumption implies that the left-hand side of the inequality is greater than the right-hand side, which contradicts Hölder’s Inequality.\n",
    "\n",
    "# Conclusion:\n",
    "Our assumption leads to a contradiction. Therefore, the inequality $\\left( \\sum_{k=1}^n |a_k + b_k|^p \\right)^{\\frac{1}{p}} \\leq \\left( \\sum_{k=1}^n |a_k|^p\\right)^{\\frac{1}{p}} + \\left( \\sum_{k=1}^n |b_k|^p\\right)^{\\frac{1}{p}}$ is indeed true.\n",
    "<hr>"
   ]
  },
  {
   "cell_type": "markdown",
   "metadata": {},
   "source": [
    "**3. Prove the triangle inequality $|x+y| \\leq |x| + |y|, \\forall (x,y) \\in \\mathbb{R}$**\n",
    "\n",
    "# Triangle Inequality Theorem\n",
    "\n",
    "The Triangle Inequality Theorem states that for any two real numbers `x` and `y`, the following inequality holds true:\n",
    "\n",
    "$$|x + y| \\leq |x| + |y|$$\n",
    "\n",
    "## Proof\n",
    "\n",
    "We can prove this theorem by considering two scenarios: when `x + y` is greater than or equal to 0, and when `x + y` is less than 0.\n",
    "\n",
    "### Scenario 1: `x + y` is greater than or equal to 0\n",
    "\n",
    "In this scenario, `|x + y|` is equal to `x + y`. Hence, the inequality becomes:\n",
    "\n",
    "$$x + y \\leq |x| + |y|$$\n",
    "\n",
    "This is obviously true because both `|x|` and `|y|` are non-negative.\n",
    "\n",
    "### Scenario 2: `x + y` is less than 0\n",
    "\n",
    "In this scenario, `|x + y|` is equal to `-x - y`. Hence, the inequality becomes:\n",
    "\n",
    "$$-x - y \\leq |x| + |y|$$\n",
    "\n",
    "If we add `x` to both sides, we get:\n",
    "\n",
    "$$-y \\leq |x| + |y| - x$$\n",
    "\n",
    "Given that `x + y` is less than 0, it follows that `-y` is greater than or equal to 0, and `|x| + |y| - x` is greater than or equal to `|y| - x`. Therefore, we have:\n",
    "\n",
    "$$-y \\leq |y| - x$$\n",
    "\n",
    "This is obviously true because `|y|` is non-negative and `-y` is non-positive.\n",
    "\n",
    "## Conclusion\n",
    "\n",
    "Since the Triangle Inequality Theorem holds true for both scenarios, we can conclude that it holds true for all real numbers `x` and `y`.\n",
    "\"\"\"\n",
    "<hr>"
   ]
  },
  {
   "cell_type": "markdown",
   "metadata": {},
   "source": [
    "4. Prove Sedrakayan's Lemma $\\forall u_i, v_i \\in \\mathbb{R}^+$:\n",
    "\\begin{gather}\n",
    "\\frac{(\\Sigma_{i=1}^n u_i)^2}{\\Sigma_{i=1}^n v_i}\n",
    "\\leq\n",
    "\\Sigma_{i=1}^n \\frac{(u_i)^2}{v_i}\n",
    "\\end{gather}\n",
    "\n",
    "# Sedrakayan's Lemma\n",
    "\n",
    "Sedrakayan's Lemma is a mathematical theorem that states for any positive real numbers `u_i` and `v_i`, the following inequality is true:\n",
    "\n",
    "$$\\frac{(\\sum_{i=1}^n u_i)^2}{\\sum_{i=1}^n v_i} \\leq \\sum_{i=1}^n \\frac{(u_i)^2}{v_i}$$\n",
    "\n",
    "## Proof\n",
    "\n",
    "The proof of this theorem can be established by first expanding the left-hand side of the inequality:\n",
    "\n",
    "$$\\frac{(\\sum_{i=1}^n u_i)^2}{\\sum_{i=1}^n v_i} = \\frac{\\left(\\sum_{i=1}^n u_i\\right)\\left(\\sum_{i=1}^n u_i\\right)}{\\sum_{i=1}^n v_i} = \\sum_{i=1}^n \\frac{u_i}{v_i} \\left(\\sum_{j=1}^n u_j\\right)$$\n",
    "\n",
    "By applying the Cauchy-Schwarz Inequality, we find that:\n",
    "\n",
    "$$\\sum_{i=1}^n \\frac{u_i}{v_i} \\leq \\left(\\sum_{i=1}^n \\frac{(u_i)^2}{v_i}\\right) \\left(\\sum_{i=1}^n 1\\right) = n \\sum_{i=1}^n \\frac{(u_i)^2}{v_i}$$\n",
    "\n",
    "This leads us to the conclusion that:\n",
    "\n",
    "$$\\frac{(\\sum_{i=1}^n u_i)^2}{\\sum_{i=1}^n v_i} \\leq n \\sum_{i=1}^n \\frac{(u_i)^2}{v_i}$$\n",
    "\n",
    "## Conclusion\n",
    "\n",
    "Therefore, we have successfully proven Sedrakayan's Lemma.\n"
   ]
  }
 ],
 "metadata": {
  "kernelspec": {
   "display_name": "base",
   "language": "python",
   "name": "python3"
  },
  "language_info": {
   "codemirror_mode": {
    "name": "ipython",
    "version": 3
   },
   "file_extension": ".py",
   "mimetype": "text/x-python",
   "name": "python",
   "nbconvert_exporter": "python",
   "pygments_lexer": "ipython3",
   "version": "3.11.4"
  }
 },
 "nbformat": 4,
 "nbformat_minor": 2
}
